SN_P.v
@@ -17,11 +17,11 @@ Import SN CCSN.
 Import PresburgerTheory PresburgerSem IntpPresburger.
 
 Lemma SN_P : forall e x y,
-  (exists hyp a b i j, 
-    x = app_esub i j (intp_fotrm a) /\
-    y = app_esub i j (intp_fotrm b) /\
+  (exists hyp a b es, 
+    x = app_esub es (intp_fotrm a) /\
+    y = app_esub es (intp_fotrm b) /\
     wf_clsd_env (intp_hyp hyp) /\
-    typ_esub e i j (intp_hyp hyp) /\
+    typ_esub e es (intp_hyp hyp) /\
     deriv hyp (eq_fotrm a b)) ->
   eq_typ e x y.
 Proof. apply SN_T. Qed.
